New replay implementation

theories/Shallow/Executor.v
@@ -394,58 +394,6 @@ Module Type ShallowExecOn
 
   End CStoreSpec.
 
-  Module Replay.
-    Import SymProp.
-    Import CPureSpec.
-
-    Definition replay_aux : forall {Σ} (ι : Valuation Σ) (s : 𝕊 Σ),
-        CPureSpec unit :=
-      fix replay {Σ} ι s :=
-        match s with
-        | SymProp.angelic_binary o1 o2 =>
-            angelic_binary (replay ι o1) (replay ι o2)
-        | SymProp.demonic_binary o1 o2 =>
-            demonic_binary (replay ι o1) (replay ι o2)
-        | SymProp.block =>
-            block
-        | SymProp.error msg =>
-            error
-        | SymProp.assertk fml msg k =>
-            bind (assert_formula (instprop fml ι))
-              (fun _ => replay ι k)
-        | SymProp.assumek fml k =>
-            bind (assume_formula (instprop fml ι))
-              (fun _ => replay ι k)
-        | SymProp.angelicv b k =>
-            bind (angelic _)
-              (fun v => replay (env.snoc ι b v) k)
-        | SymProp.demonicv b k =>
-            bind (demonic _)
-              (fun v => replay (env.snoc ι b v ) k)
-        | @SymProp.assert_vareq _ x σ xIn t msg k =>
-            let ι' := env.remove (x ∷ σ) ι xIn in
-            let x' := ι.[? x∷σ] in
-            let t' := inst t ι' in
-            bind (assert_formula (x' = t'))
-                 (fun _ => replay ι' k)
-        | @SymProp.assume_vareq _ x σ xIn t k =>
-            let ι' := env.remove (x ∷ σ) ι xIn in
-            let x' := ι.[? x∷σ] in
-            let t' := inst t ι' in
-            bind (assume_formula (x' = t'))
-                 (fun _ => replay ι' k)
-        | SymProp.pattern_match s pat rhs =>
-            error
-        | SymProp.pattern_match_var x pat rhs =>
-            error
-        | SymProp.debug b k =>
-            replay ι k
-        end.
-
-    Definition replay {Σ} (ι : Valuation Σ) (s : 𝕊 Σ) : Prop :=
-      replay_aux ι s (fun _ => TRUE).
-  End Replay.
-
   Module Shallow.
 
     Definition ValidContractWithFuel {Δ τ} (fuel : nat) (c : SepContract Δ τ) (body : Stm Δ τ) : Prop :=
