theories/Symbolic/Monads.v
@@ -590,6 +590,57 @@ Module Type SymbolicMonadsOn (Import B : Base) (Import P : PredicateKit B)
         | _ , _ => error msg⟨θ1⟩
         end.
 
+    Definition replay_aux :
+      forall {Σ} (s : 𝕊 Σ), ⊢ Sub Σ -> SPureSpec Unit :=
+      fix replay {Σ} s {w0} δ {struct s} :=
+        match s with
+        | SymProp.angelic_binary o1 o2 =>
+            SPureSpec.angelic_binary (replay o1 δ) (replay o2 δ)
+        | SymProp.demonic_binary o1 o2 =>
+            SPureSpec.demonic_binary (replay o1 δ) (replay o2 δ)
+        | SymProp.block => block
+        | SymProp.error msg =>
+            error (subst msg δ)
+        | SymProp.assertk fml msg k =>
+            ⟨ θ ⟩ _ <- assert_formula (subst msg δ) (subst fml δ) ;;
+            replay k (persist δ θ)
+        | SymProp.assumek fml k =>
+            ⟨ θ ⟩ _ <- assume_formula (subst fml δ) ;;
+            replay k (persist δ θ)
+        | SymProp.angelicv b k =>
+            ⟨ θ ⟩ t <- angelic (Some (name b)) (type b) ;;
+            replay k (env.snoc (persist δ θ) b t)
+        | SymProp.demonicv b k =>
+            ⟨ θ ⟩ t <- demonic (Some (name b)) (type b) ;;
+            replay k (env.snoc (persist δ θ) b t)
+        | SymProp.assert_vareq x t msg k =>
+            let ζ    := sub_shift (b:=x∷_) _ in
+            let msg  := subst msg ζ in
+            let fml  := formula_relop bop.eq (subst t ζ) (term_var x) in
+            ⟨ θ ⟩ _ <- assert_formula (subst msg δ) (subst fml δ) ;;
+            replay k (env.remove (x∷_) δ⟨θ⟩ _)
+        | SymProp.assume_vareq x t k =>
+            let ζ    := sub_shift (b:=x∷_) _ in
+            let fml  := formula_relop bop.eq (subst t ζ) (term_var x) in
+            ⟨ θ ⟩ _ <- assume_formula (subst fml δ) ;;
+            replay k (env.remove (x∷_) δ⟨θ⟩ _)
+        | SymProp.pattern_match s pat rhs =>
+            error (amsg.mk tt)
+        (* FIXME *)
+        (* ⟨ θ ⟩ '(existT pc δpc) <- new_pattern_match id pat (subst s δ) ;; *)
+        (* replay (rhs pc) (persist δ θ ►► δpc) *)
+        | SymProp.pattern_match_var x pat rhs =>
+            error (amsg.mk tt)
+        (* FIXME *)
+        (* ⟨ θ ⟩ '(existT pc δpc) <- new_pattern_match id pat (subst (term_var x) δ) ;; *)
+        (* replay (rhs pc) (env.remove _ (δ⟨θ⟩ ►► δpc) _) *)
+        | SymProp.debug msg k =>
+            debug (subst msg δ) (replay k δ)
+        end.
+
+    Definition replay : ⊢ 𝕊 -> 𝕊 :=
+      fun w P => run (replay_aux P (sub_id w)).
+
   End SPureSpec.
   Export (hints) SPureSpec.
 
