theories/Symbolic/Soundness.v
@@ -1096,199 +1096,12 @@ Module Soundness
     reflexivity.
   Qed.
 
-  Lemma refine_replay_aux_debug :
-    forall
-      {Σ}
-      {w : World}
-      (b : AMessage Σ)
-      (s : 𝕊 Σ)
-      (ω : {| wctx := Σ; wco := [ctx] |} ⊒ w)
-      (ι : Valuation w)
-      (i : Valuation Σ),
-      i = inst (sub_acc ω) ι ->
-      ℛ⟦RPureSpec RUnit⟧@{ι} (Replay.replay_aux s ω) (SHAL.Replay.replay_aux i s) ->
-      ℛ⟦RPureSpec RUnit⟧@{ι} (fun P => debug (subst b (sub_acc ω)) (Replay.replay_aux s ω P)) (SHAL.Replay.replay_aux i s).
+  Lemma replay_sound {w : World} (s : 𝕊 w) ι (Hpc : instprop (wco w) ι) :
+    safe (SPureSpec.replay s) ι -> safe s ι.
   Proof.
-    intros Σ w b s ω ι i Hi H.
-    intros ta a ? Hdebug.
-    cbn in Hdebug.
-    rewrite debug_equiv in Hdebug.
-    apply H with (ta := ta); auto.
-  Qed.
-
-  Lemma refine_replay_aux {Σ} (s : 𝕊 Σ) {w : World} :
-    forall
-      (ω : MkWorld Σ [ctx] ⊒ w)
-      (ι : Valuation w)
-      (i : Valuation Σ)
-      (Hpc0 : instprop (wco w) ι),
-      i = inst (sub_acc ω) ι ->
-      ℛ⟦RPureSpec RUnit⟧@{ι} (Replay.replay_aux s ω) (SHAL.Replay.replay_aux i s).
-  Proof.
-    revert w; induction s; intros * Hpc Hi; cbn - [RSat wctx Val].
-    - apply RPureSpec.refine_angelic_binary; auto.
-    - apply RPureSpec.refine_demonic_binary; auto.
-    - apply RPureSpec.refine_error; auto.
-    - apply RPureSpec.refine_block; auto.
-    - apply RPureSpec.refine_bind; auto.
-      + apply RPureSpec.refine_assert_formula; auto.
-        eapply refine_formula_persist; eauto.
-        now cbn.
-      + intros w2 ω12 ι2 Hι2 Hpc2 _ _ _. apply IHs; auto.
-        subst. now rewrite sub_acc_trans, inst_subst, <- inst_persist.
-    - apply RPureSpec.refine_bind; auto.
-      + apply RPureSpec.refine_assume_formula; auto.
-        eapply refine_formula_persist; eauto.
-        now cbn.
-      + intros w2 ω12 ι2 Hι2 Hpc2 _ _ _. apply IHs; auto.
-        subst. now rewrite sub_acc_trans, inst_subst, <- inst_persist.
-    - intros ? ? Hrefine; cbn - [RSat wctx Val].
-      cbn.
-      intros [v H].
-      unfold CPureSpec.bind, CPureSpec.angelic.
-      exists v.
-      unshelve eapply (IHs _ _ _ _ _ _ _ _ _ H).
-      + cbn.
-        now rewrite instprop_subst, inst_sub_wk1.
-      +  cbn [sub_acc].
-         subst.
-         now rewrite <- inst_sub_up1.
-      + unshelve eapply (refine_four _ _ Hrefine).
-        cbn. now rewrite inst_sub_wk1.
-    - intros ? ? Hrefine; cbn - [RSat wctx Val].
-      cbn.
-      intros H v.
-      unshelve eapply (IHs _ _ _ _ _ _ _ _ _ (H v)).
-      +  cbn.
-         now rewrite instprop_subst, inst_sub_wk1.
-      +  cbn [sub_acc].
-         subst.
-         now rewrite <- inst_sub_up1.
-      + unshelve eapply (refine_four _ _ Hrefine).
-        cbn. now rewrite inst_sub_wk1.
-    - apply RPureSpec.refine_bind; auto.
-      + apply RPureSpec.refine_assert_formula; auto.
-        cbn. subst.
-        now rewrite <- inst_sub_shift, <- ?inst_subst, <- subst_sub_comp, <- inst_lookup.
-      + intros w2 ω12 ι2 Hι2 Hpc2 _ _ _. apply IHs; auto.
-        subst. rewrite sub_acc_trans. cbn [sub_acc]. now rewrite ?inst_subst, <- inst_sub_shift.
-    - apply RPureSpec.refine_bind; auto.
-      + apply RPureSpec.refine_assume_formula; auto.
-        cbn. subst.
-        now rewrite <- inst_sub_shift, <- ?inst_subst, <- subst_sub_comp, <- inst_lookup.
-      + intros w2 ω12 ι2 Hι2 Hpc2 _ _ _. apply IHs; auto.
-        subst. rewrite sub_acc_trans. cbn [sub_acc]. now rewrite ?inst_subst, <- inst_sub_shift.
-    - now cbn.
-    - now cbn.
-    - apply refine_replay_aux_debug; auto.
-  Qed.
-
-  Lemma refine_replay {Σ} (s : 𝕊 Σ) {w : World} :
-    forall
-      (ω : MkWorld Σ [ctx] ⊒ w)
-      (ι : Valuation w),
-      let i := inst (sub_acc ω) ι in
-      ℛ⟦ℙ⟧@{i} (Replay.replay s) (SHAL.Replay.replay i s).
-  Proof.
-    intros.
-    apply refine_replay_aux.
-    - now cbn.
-    - cbn [sub_acc sub_id].
-      symmetry.
-      apply inst_sub_id.
-    - now cbn.
-  Qed.
-
-  Lemma shallow_replay_complete {Σ} (s : 𝕊 Σ) {w : World} :
-    forall
-      (ω : MkWorld Σ [ctx] ⊒ w)
-      (ι : Valuation w)
-      (i : Valuation Σ)
-      (Hpc0 : instprop (wco w) ι),
-      i = inst (sub_acc ω) ι ->
-      SHAL.Replay.replay i s ->
-      safe s i.
-  Proof.
-    revert w; induction s; intros w ω ι i Hpc0 Hi Hreplay.
-    - destruct Hreplay as [H|H].
-      + left.
-        apply (IHs1 w ω ι i Hpc0 Hi H).
-      + right.
-        apply (IHs2 w ω ι i Hpc0 Hi H).
-    - destruct Hreplay as [Hs1 Hs2].
-      split.
-      + apply (IHs1 w ω ι i Hpc0 Hi Hs1).
-      + apply (IHs2 w ω ι i Hpc0 Hi Hs2).
-    - auto.
-    - auto.
-    - cbn in Hreplay.
-      unfold CPureSpec.bind, CPureSpec.assert_formula in Hreplay.
-      destruct Hreplay as [Hfml Hs].
-      split; auto.
-      apply (IHs w ω ι i Hpc0 Hi Hs).
-    - cbn in Hreplay.
-      unfold CPureSpec.bind, CPureSpec.assume_formula in Hreplay.
-      intros Hfml.
-      apply (IHs w ω ι i Hpc0 Hi (Hreplay Hfml)).
-    - cbn in Hreplay.
-      unfold CPureSpec.bind, CPureSpec.angelic in Hreplay.
-      destruct Hreplay as [v Hreplay].
-      exists v.
-      unshelve eapply (IHs (wsnoc w b) _ ι.[b ↦ v] _ _ _ Hreplay).
-      + apply acc_sub with (ζ := sub_up1 (sub_acc ω)).
-        apply Entailment.entails_nil.
-      + cbn.
-        now rewrite instprop_subst, inst_sub_wk1.
-      + subst.
-        now rewrite <- inst_sub_up1.
-    - cbn in Hreplay.
-      unfold CPureSpec.bind, CPureSpec.demonic in Hreplay.
-      intros v.
-      unshelve eapply (IHs (wsnoc w b) _ ι.[b ↦ v] _ _ _ (Hreplay v)).
-      + apply acc_sub with (ζ := sub_up1 (sub_acc ω)).
-        apply Entailment.entails_nil.
-      + cbn.
-        now rewrite instprop_subst, inst_sub_wk1.
-      + subst.
-        now rewrite <- inst_sub_up1.
-    - cbn in Hreplay.
-      unfold CPureSpec.bind, CPureSpec.assert_formula in Hreplay.
-      destruct Hreplay as [Heq Hreplay].
-      split; auto.
-      unshelve eapply (IHs _ _ (inst (sub_acc ω) ι) _ _ _ Hreplay).
-      + apply acc_sub with (ζ := sub_shift xIn).
-        apply Entailment.entails_nil.
-      + now cbn.
-      + rewrite <- inst_sub_shift.
-        cbn [sub_acc].
-        now subst.
-    - cbn in Hreplay.
-      unfold CPureSpec.bind, CPureSpec.assume_formula in Hreplay.
-      intros Heq.
-      unshelve eapply (IHs _ _ (inst (sub_acc ω) ι) _ _ _ (Hreplay Heq)).
-      + apply acc_sub with (ζ := sub_shift xIn).
-        apply Entailment.entails_nil.
-      + now cbn.
-      + rewrite <- inst_sub_shift.
-        cbn [sub_acc].
-        now subst.
-    - now cbn in Hreplay.
-    - now cbn in Hreplay.
-    - cbn in Hreplay.
-      apply (IHs _ _ ι _ Hpc0 Hi Hreplay).
-  Qed.
-
-  Lemma replay_sound_nil (s : 𝕊 [ctx]) :
-    forall ι,
-      safe (Replay.replay s) ι -> safe s ι.
-  Proof.
-    intros ι H.
-    destruct (env.view ι).
-    rewrite <- ?safe_debug_safe in H.
-    rewrite <- (@wsafe_safe wnil _ [env]) in H.
-    apply (@refine_replay [ctx] s wnil acc_refl [env]) in H.
-    assert (Hwco: instprop (wco wnil) [env]) by now cbn.
-    apply (@shallow_replay_complete [ctx] s wnil acc_refl [env] [env] Hwco eq_refl H).
+    intros H.
+    apply CPureSpec.replay_sound, RPureSpec.refine_replay; auto.
+    now rewrite wsafe_safe, safe_debug_safe.
   Qed.
 
   Lemma symbolic_vcgen_soundness {Γ τ} (c : SepContract Γ τ) (body : Stm Γ τ) :
@@ -1296,8 +1109,9 @@ Module Soundness
     Shallow.ValidContract c body.
   Proof.
     unfold Symbolic.ValidContract. intros [Hwp%postprocess_sound].
-    apply replay_sound_nil in Hwp. apply postprocess_sound in Hwp.
-    apply refine_vcgen. now rewrite wsafe_safe, safe_debug_safe.
+    apply (replay_sound (w:=wnil)) in Hwp; [|easy].
+    apply postprocess_sound in Hwp. apply refine_vcgen.
+    now rewrite wsafe_safe, safe_debug_safe.
   Qed.
 
   Lemma symbolic_vcgen_fuel_soundness {Γ τ} (fuel : nat) (c : SepContract Γ τ) (body : Stm Γ τ) :
@@ -1305,8 +1119,9 @@ Module Soundness
     Shallow.ValidContractWithFuel fuel c body.
   Proof.
     unfold Symbolic.ValidContractWithFuel. intros [Hwp%postprocess_sound].
-    apply replay_sound_nil in Hwp. apply postprocess_sound in Hwp.
-    apply refine_vcgen. now rewrite wsafe_safe, safe_debug_safe.
+    apply (replay_sound (w:=wnil)) in Hwp; [|easy].
+    apply postprocess_sound in Hwp. apply refine_vcgen.
+    now rewrite wsafe_safe, safe_debug_safe.
   Qed.
 
   (* Print Assumptions symbolic_vcgen_soundness. *)
